pagedbetree is code complete; let's try to refine it

Splinter/Betree/PagedBetree.i.dfy
@@ -3,23 +3,10 @@
 
 include "../CoordinationLayer/AbstractMap.i.dfy"
 
-module ChildMapMod refines TotalMapMod {
+module PagedBetree
+{
   import opened Options
   import opened KeyType
-
-  type NodeType(!new,==)   // placeholder for Betree down where we define it.
-
-  type K = Key
-  type V = Option<NodeType>
-  predicate TerminalValue(v: V) { true }
-  function DefaultV() : V { None }
-
-  type ChildMap = TotalMap
-}
-
-module PagedBetree
-  refines ChildMapMod // refinement here because that's the only way to supply ChildMapMod.NodeType
-{
   import opened StampedMapMod
   import TotalKMMapMod
   import opened ValueMessage
@@ -31,16 +18,21 @@ module PagedBetree
       QueryLabel(endLsn: LSN, key: Key, value: Value)
     | PutLabel(puts: MsgHistory)
     | QueryEndLsnLabel(endLsn: LSN)
-    | FreezeAsLabel(stampedMap: StampedMap)
+    | FreezeAsLabel(stampedBetree: StampedBetree)
     | InternalLabel()
 
-  datatype Buffer = Buffer(filter: set<Key>, mapp: map<Key, Message>)
+  datatype Buffer = Buffer(filter: iset<Key>, mapp: map<Key, Message>)
   {
     function Query(key: Key) : Message
     {
       if key in filter && key in mapp
       then mapp[key]
       else Update(NopDelta())
+    }
+
+    function ApplyFilter(accept: iset<Key>) : Buffer
+    {
+      Buffer(filter * accept, mapp)
     }
   }
 
@@ -58,19 +50,124 @@ module PagedBetree
     {
       QueryUpTo(key, |buffers|)
     }
+
+    function ApplyFilter(accept: iset<Key>) : BufferStack
+    {
+      BufferStack(seq(|buffers|, i requires 0<=i<|buffers| => buffers[i].ApplyFilter(accept)))
+    }
+
+    function PrependBufferStack(newBuffers: BufferStack) : BufferStack
+    {
+      BufferStack(newBuffers.buffers + this.buffers)
+    }
+
+    predicate Equivalent(other: BufferStack)
+    {
+      forall k | AnyKey(k) :: Query(k) == other.Query(k)
+    }
   }
 
-  type NodeType = BetreeNode  // Tell ChildMapMod about BetreeNodes
+  // I'd prefer to instantiate TotalMapMod here, but rank_is_less_than doesn't
+  // make it through the module refinement, so I can't prove decreases when I
+  // recursively walk down the BetreeNode. So I do it manually instead.
+  predicate AnyKey(key: Key) { true }
+  predicate Total(keys: iset<Key>) {
+    forall k | AnyKey(k) :: k in keys
+  }
+  function AllKeys() : (out: iset<Key>)
+    ensures Total(out)
+  {
+    iset k | AnyKey(k)
+  }
+  datatype ChildMap = ChildMap(mapp: imap<Key, BetreeNode>) {
+    predicate WF() {
+      && Total(mapp.Keys)
+      && (forall k | AnyKey(k) :: mapp[k].WF())
+    }
+  }
+  
+  function EmptyChildMap() : (out: ChildMap)
+    ensures out.WF()
+  {
+    var mapp := imap key | AnyKey(key) :: Nil;
+    ChildMap(mapp)
+  }
+  
+  datatype Domain = DomainTODO  // TODO placeholder
 
-  datatype BetreeNode = BetreeNode(
-    domain: set<Key>,
+  datatype BetreeNode = Nil | BetreeNode(
+    domain: Domain,
     children: ChildMap,
-    sillychildren: imap<Key, Option<BetreeNode>>,
     buffers: BufferStack)
   {
     predicate WF() {
-      && true
+      && (BetreeNode? ==> children.WF())
     }
+
+    function PrependBufferStack(bufferStack: BufferStack) : (out: BetreeNode)
+      requires WF()
+      requires BetreeNode?
+      ensures out.WF()
+    {
+      BetreeNode(DomainTODO, children, buffers.PrependBufferStack(bufferStack))
+    }
+
+    function Split(leftKeys: iset<Key>) : (out: BetreeNode)
+      requires WF()
+      requires BetreeNode?
+      ensures out.WF()
+    {
+      assert children.WF(); // trigger
+      var leftMapp := imap key | AnyKey(key) :: if key in leftKeys then children.mapp[key] else Nil;
+      var leftNode := BetreeNode(DomainTODO, ChildMap(leftMapp), BufferStack([]));
+      assert leftNode.WF();
+
+      var rightMapp := imap key | AnyKey(key) :: if key in leftKeys then Nil else children.mapp[key];
+      var rightNode := BetreeNode(DomainTODO, ChildMap(rightMapp), BufferStack([]));
+      assert rightNode.WF();
+
+      var mapp := imap key | AnyKey(key) :: if key in leftKeys then leftNode else rightNode;
+      BetreeNode(DomainTODO, ChildMap(mapp), buffers)
+    }
+
+    function Promote() : BetreeNode
+    {
+      if Nil? then BetreeNode(DomainTODO, EmptyChildMap(), BufferStack([])) else this
+    }
+
+    function Flush(downKeys: iset<Key>) : (out: BetreeNode)
+      requires WF()
+      requires BetreeNode?
+      ensures out.WF()
+    {
+      var keptBuffers := buffers.ApplyFilter(AllKeys() - downKeys);
+      var movedBuffers := buffers.ApplyFilter(downKeys);
+      assert children.WF();
+      var outChildren := ChildMap(imap key | AnyKey(key)
+        :: if key in downKeys
+          then children.mapp[key].Promote().PrependBufferStack(movedBuffers)
+          else children.mapp[key]);
+      assert outChildren.WF();
+      var out := BetreeNode(DomainTODO, outChildren, keptBuffers);
+      assert out.WF();
+      out
+    }
+
+    predicate EquivalentBufferCompaction(other: BetreeNode)
+    {
+      && WF()
+      && other.WF()
+      && Promote().buffers.Equivalent(other.Promote().buffers)
+      // Can only make a local change; entirety of children subtrees are identical.
+      && Promote().children == other.Promote().children
+    }
+  }
+
+  function EmptyRoot() : (out: BetreeNode)
+    ensures out.WF()
+  {
+    BetreeNode(DomainTODO, EmptyChildMap(), BufferStack([])
+    )
   }
 
   datatype QueryReceiptLine = QueryReceiptLine(
@@ -79,13 +176,14 @@ module PagedBetree
   {
     predicate WF()
     {
-      result.Define?
+      && node.BetreeNode?
+      && result.Define?
     }
   }
 
   datatype QueryReceipt = QueryReceipt(
     key: Key,
-    root: Option<BetreeNode>,
+    root: BetreeNode,
     lines: seq<QueryReceiptLine>)
   {
     function ResultAt(i: nat) : Message
@@ -94,7 +192,13 @@ module PagedBetree
       if i<|lines| then lines[i].result else Define(DefaultValue())
     }
 
+    predicate AllLinesWF()
+    {
+      && (forall i:nat | i < |lines| :: lines[i].WF())
+    }
+
     predicate LinkedAt(i: nat)
+      requires AllLinesWF()
       requires i < |lines|
     {
       lines[i].result == Merge(lines[i].node.buffers.Query(key), ResultAt(i+1))
@@ -102,8 +206,8 @@ module PagedBetree
 
     predicate Valid()
     {
-      && (if root.None? then |lines| == 0 else 0 < |lines| && lines[0].node == root.value)
-      && (forall i:nat | i < |lines| :: lines[i].WF())
+      && (if root.Nil? then |lines| == 0 else 0 < |lines| && lines[0].node == root)
+      && AllLinesWF()
       && (forall i:nat | i < |lines| :: LinkedAt(i))
     }
 
@@ -111,34 +215,46 @@ module PagedBetree
     {
       ResultAt(0)
     }
+
+    predicate ValidFor(root: BetreeNode, key: Key)
+    {
+      && Valid()
+      && this.root == root
+      && this.key == key
+    }
   }
 
   // Constructive evidence that a Valid QueryReceipt exists for every key.
-  function BuildQueryReceipt(node: Option<BetreeNode>, key: Key) : (out: QueryReceipt)
+  function BuildQueryReceipt(node: BetreeNode, key: Key) : (out: QueryReceipt)
+    requires node.WF()
     ensures out.key == key
     ensures out.Valid()
     decreases node
   {
-    if node.None?
+    if node.Nil?
     then QueryReceipt(key, node, [])
     else
-      assert AnyKey(key);
-      //var childReceipt := BuildQueryReceipt(node.value.children[key], key);
-      assume key in node.value.sillychildren;
-      var childReceipt := BuildQueryReceipt(node.value.sillychildren[key], key);
-      var thisMessage := node.value.buffers.Query(key);
-      var topLine := QueryReceiptLine(node.value, Merge(thisMessage, childReceipt.Result()));
+      assert node.children.WF();  // trigger
+      var childReceipt := BuildQueryReceipt(node.children.mapp[key], key);
+      var thisMessage := node.buffers.Query(key);
+      var topLine := QueryReceiptLine(node, Merge(thisMessage, childReceipt.Result()));
       var receipt := QueryReceipt(key, node, [topLine] + childReceipt.lines);
       assert receipt.LinkedAt(0);
-      assume receipt.Valid();
+      assert forall i | 0<i<|receipt.lines| :: childReceipt.LinkedAt(i-1) && receipt.LinkedAt(i); // trigger Valid
       receipt
   }
 
   datatype StampedBetree = StampedBetree(
-    root: Option<BetreeNode>,
+    root: BetreeNode,
     seqEnd: LSN)
   {
+    predicate WF()
+    {
+      root.WF()
+    }
+    
     function I() : StampedMap
+      requires WF()
     {
       var mi := imap key | AnyKey(key) :: BuildQueryReceipt(root, key).Result();
       assert TotalKMMapMod.TotalMapIsFull(mi);
@@ -162,6 +278,11 @@ module PagedBetree
       if puts.IsEmpty() then this
       else ApplyPuts(puts.DiscardRecent(puts.seqEnd-1)).ApplyPut(puts.msgs[puts.seqEnd-1])
     }
+
+    function Query(key: Key) : Message
+    {
+      if key in mapp then mapp[key] else Update(NopDelta())
+    }
   }
 
   function EmptyMemtable(lsn: LSN) : Memtable
@@ -173,11 +294,17 @@ module PagedBetree
     memtable: Memtable,
     stampedBetree: StampedBetree)
   {
+    predicate WF() {
+      && stampedBetree.WF()
+    }
   }
 
-  predicate Query(v: Variables, v': Variables, lbl: TransitionLabel)
+  predicate Query(v: Variables, v': Variables, lbl: TransitionLabel, receipt: QueryReceipt)
   {
-    true
+    && lbl.QueryLabel?
+    && lbl.endLsn == v.stampedBetree.seqEnd
+    && receipt.ValidFor(v.stampedBetree.root, lbl.key)
+    && Define(lbl.value) == Merge(v.memtable.Query(lbl.key), receipt.Result())
   }
 
   predicate Put(v: Variables, v': Variables, lbl: TransitionLabel)
@@ -185,35 +312,114 @@ module PagedBetree
     && lbl.PutLabel?
     && lbl.puts.WF()
     && lbl.puts.seqStart == v.memtable.seqEnd
-    && v' == v.(memtable := v.memtable.ApplyPuts(lbl.puts))
+    && v' == v.(
+        memtable := v.memtable.ApplyPuts(lbl.puts)
+      )
   }
 
   predicate QueryEndLsn(v: Variables, v': Variables, lbl: TransitionLabel)
   {
-    true
+    && lbl.QueryEndLsnLabel?
+    && lbl.endLsn == v.stampedBetree.seqEnd
   }
 
   predicate FreezeAs(v: Variables, v': Variables, lbl: TransitionLabel, stampedBetree: StampedBetree)
   {
     && lbl.FreezeAsLabel?
-    && stampedBetree.I() == lbl.stampedMap
     && stampedBetree == v.stampedBetree
     && v' == v
   }
 
-  predicate InternalSplit(v: Variables, v': Variables, lbl: TransitionLabel)
+  predicate InternalFlushMemtable(v: Variables, v': Variables, lbl: TransitionLabel)
   {
-    true
+    && v.WF()
+    && var newBuffer := Buffer(AllKeys(), v.memtable.mapp);
+    && var rootBase := if v.stampedBetree.root.Nil? then EmptyRoot() else v.stampedBetree.root;
+    && v' == v.(
+        memtable := EmptyMemtable(v.memtable.seqEnd),
+        stampedBetree := StampedBetree(rootBase.PrependBufferStack(BufferStack([newBuffer])), v.memtable.seqEnd)
+      )
+  }
+  
+  datatype Path = Path(node: BetreeNode, key: Key, depth: nat)
+  {
+    function Subpath() : (out: Path)
+      requires 0 < depth
+      requires node.WF()
+      requires node.BetreeNode?
+    {
+      assert node.children.WF();
+      Path(node.children.mapp[key], key, depth-1)
+    }
+
+    predicate Valid()
+      decreases depth
+    {
+      && node.WF()
+      && node.BetreeNode?
+      //&& (0 < depth ==> Path(node.children[key], key, depth-1).Valid())
+      && (0 < depth ==> Subpath().Valid())
+    }
+
+    function Node() : (out: BetreeNode)
+      requires Valid()
+      ensures out.WF()
+      ensures out.BetreeNode?
+      decreases depth
+    {
+      if 0 == depth
+      then node
+      else Subpath().Node()
+    }
+
+    function Substitute(replacement: BetreeNode) : (out: BetreeNode)
+      requires Valid()
+      decreases depth
+    {
+      if 0 == depth
+      then replacement
+      else Subpath().Substitute(replacement)
+    }
   }
 
-  predicate InternalFlush(v: Variables, v': Variables, lbl: TransitionLabel)
+  predicate InternalSplit(v: Variables, v': Variables, lbl: TransitionLabel, step: Step)
   {
-    true
+    && step.InternalSplitStep?
+    && step.path.Valid()
+    && step.path.node == v.stampedBetree.root
+    && v' == v.(
+        stampedBetree := v.stampedBetree.(
+          root := step.path.Substitute(step.path.Node().Split(step.leftKeys))
+        )
+      )
   }
 
-  predicate InternalCompact(v: Variables, v': Variables, lbl: TransitionLabel)
+  predicate InternalFlush(v: Variables, v': Variables, lbl: TransitionLabel, step: Step)
   {
-    true
+    && step.InternalFlushStep?
+    && step.path.Valid()
+    && step.path.node == v.stampedBetree.root
+    && v' == v.(
+        stampedBetree := v.stampedBetree.(
+          root := step.path.Substitute(step.path.Node().Flush(step.downKeys))
+        )
+      )
+  }
+
+  // NB we tell you exactly how to Split and Flush, but leave lots of
+  // nondetermistic freedom in the description of Compact.
+  predicate InternalCompact(v: Variables, v': Variables, lbl: TransitionLabel, step: Step)
+  {
+    && step.InternalCompactStep?
+    && step.path.Valid()
+    && step.path.node == v.stampedBetree.root
+    && step.compactedNode.WF()
+    && step.path.Node().EquivalentBufferCompaction(step.compactedNode)
+    && v' == v.(
+        stampedBetree := v.stampedBetree.(
+          root := step.path.Substitute(step.compactedNode)
+        )
+      )
   }
 
   // public:
@@ -224,24 +430,24 @@ module PagedBetree
   }
 
   datatype Step =
-      QueryStep()
+      QueryStep(receipt: QueryReceipt)
     | PutStep()
     | QueryEndLsnStep()
     | FreezeAsStep(stampedBetree: StampedBetree)
-    | InternalSplitStep()
-    | InternalFlushStep()
-    | InternalCompactStep()
+    | InternalSplitStep(path: Path, leftKeys: iset<Key>)
+    | InternalFlushStep(path: Path, downKeys: iset<Key>)
+    | InternalCompactStep(path: Path, compactedNode: BetreeNode)
 
   predicate NextStep(v: Variables, v': Variables, lbl: TransitionLabel, step: Step)
   {
     match step {
-      case QueryStep() => Query(v, v', lbl)
+      case QueryStep(receipt) => Query(v, v', lbl, receipt)
       case PutStep() => Put(v, v', lbl)
       case QueryEndLsnStep() => QueryEndLsn(v, v', lbl)
       case FreezeAsStep(stampedBetree) => FreezeAs(v, v', lbl, stampedBetree)
-      case InternalSplitStep() => InternalSplit(v, v', lbl)
-      case InternalFlushStep() => InternalFlush(v, v', lbl)
-      case InternalCompactStep() => InternalCompact(v, v', lbl)
+      case InternalSplitStep(_, _) => InternalSplit(v, v', lbl, step)
+      case InternalFlushStep(_, _) => InternalFlush(v, v', lbl, step)
+      case InternalCompactStep(_, _) => InternalCompact(v, v', lbl, step)
     }
   }
 
